feat: faster, linear HashMap.alter and modify (#6573)
This PR replaces the existing implementations of `(D)HashMap.alter` and
`(D)HashMap.modify` with primitive, more efficient ones and in
particular provides proofs that they yield well-formed hash maps (`WF`
typeclass).

---------

Co-authored-by: Paul Reichert <6992158+datokrat@users.noreply.github.com>

src/Std/Data/DHashMap/Internal/AssocList/Basic.lean
@@ -170,6 +170,63 @@ def erase [BEq α] (a : α) : AssocList α β → AssocList α β
   | cons k v l => bif k == a then l else cons k v (l.erase a)
 
 /-- Internal implementation detail of the hash map -/
+def modify [BEq α] [LawfulBEq α] (a : α) (f : β a → β a) :
+    AssocList α β → AssocList α β
+  | nil => nil
+  | cons k v l =>
+    if h : k == a then
+      have h' : k = a := eq_of_beq h
+      let b := f (cast (congrArg β h') v)
+      cons a b l
+    else
+      cons k v (modify a f l)
+
+/-- Internal implementation detail of the hash map -/
+def alter [BEq α] [LawfulBEq α] (a : α) (f : Option (β a) → Option (β a)) :
+    AssocList α β → AssocList α β
+  | nil => match f none with
+    | none => nil
+    | some b => cons a b nil
+  | cons k v l =>
+    if h : k == a then
+      have h' : k = a := eq_of_beq h
+      match f (some (cast (congrArg β h') v)) with
+      | none => l
+      | some b => cons a b l
+    else
+      let tail := alter a f l
+      cons k v tail
+
+namespace Const
+
+/-- Internal implementation detail of the hash map -/
+def modify [BEq α] {β : Type v} (a : α) (f : β → β) :
+    AssocList α (fun _ => β) → AssocList α (fun _ => β)
+  | nil => nil
+  | cons k v l =>
+    if k == a then
+      cons a (f v) l
+    else
+      cons k v (modify a f l)
+
+/-- Internal implementation detail of the hash map -/
+def alter [BEq α] {β : Type v} (a : α) (f : Option β → Option β) :
+    AssocList α (fun _ => β) → AssocList α (fun _ => β)
+  | nil => match f none with
+    | none => nil
+    | some b => AssocList.cons a b nil
+  | cons k v l =>
+    if k == a then
+      match f v with
+      | none => l
+      | some b => cons a b l
+    else
+      let tail := alter a f l
+      cons k v tail
+
+end Const
+
+/-- Internal implementation detail of the hash map -/
 @[inline] def filterMap (f : (a : α) → β a → Option (γ a)) :
     AssocList α β → AssocList α γ :=
   go .nil
